Misc/Splitter.v
@@ -1,0 +1,48 @@
+Require Import Coq.omega.Omega.
+
+Module Splitter.
+
+  Record t : Type := mkT {
+    get : nat -> nat ;
+    injective: forall (m n:nat),
+      m <> n -> get m <> get n
+  }.
+
+  Lemma id_injective:
+    forall (m n:nat),
+    m <> n -> m <> n.
+  Proof.
+    tauto.
+  Qed.
+
+  Lemma left_injective:
+    forall (acc:t) (m n:nat),
+    m <> n -> (fun n => (get acc) (2*n)) m <> (fun n => (get acc) (2*n)) n.
+  Proof.
+    intros.
+    simpl.
+    apply (injective acc).
+    omega.
+  Qed.
+
+  Lemma right_injective:
+    forall (acc:t) (m n:nat),
+    m <> n -> (fun n => (get acc) (2*n+1)) m <> (fun n => (get acc) (2*n+1)) n.
+  Proof.
+    intros.
+    simpl.
+    apply (injective acc).
+    omega.
+  Qed.
+
+  Definition empty : t := mkT (fun n => n) id_injective.
+
+  Definition left (acc:t) : t := mkT 
+    (fun n => (get acc) (2*n)) (left_injective acc).
+
+  Definition right (acc:t) : t := mkT
+    (fun n => (get acc) (2*n+1)) (right_injective acc).
+
+  Definition split (acc:t) : t * t := (left acc, right acc).
+
+End Splitter.
